Towards substitutions

src/Language.v
@@ -3,12 +3,7 @@
 (* ON SEPERATION LOGIC *)
 (* Author: Hans-Dieter A. Hiep *)
 
-Require Import FunctionalExtensionality.
-Require Import PropExtensionality.
-Require Import List.
-Require Import ZArith.
-
-Require Import OnSeparationLogic.Heap.
+Require Export OnSeparationLogic.Heap.
 
 Module Language (Export HS: HeapSig).
 
@@ -109,6 +104,15 @@ exfalso. apply H; assumption.
 reflexivity.
 Qed.
 
+Proposition store_update_id (s: store) (x: V):
+  store_update s x (s x) = s.
+apply functional_extensionality; intro.
+unfold store_update.
+destruct (Nat.eq_dec x x0).
+rewrite e; reflexivity.
+reflexivity.
+Qed.
+
 Definition eq_restr (s t: store) (z: list V): Prop :=
   forall (x: V), In x z -> s x = t x.
 
@@ -116,6 +120,11 @@ Proposition eq_restr_split (s t: store) (xs ys: list V):
   eq_restr s t (xs ++ ys) -> eq_restr s t xs /\ eq_restr s t ys.
 unfold eq_restr; intro; split; intros;
 apply H; apply in_or_app; auto.
+Qed.
+
+Proposition eq_restr_comm (s t: store) (xs: list V):
+  eq_restr s t xs -> eq_restr t s xs.
+unfold eq_restr; intros; symmetry; apply H; assumption.
 Qed.
 
 (* Expressions and guards are shallow, but finitely based *)
@@ -143,6 +152,39 @@ Definition var_expr (x: V): expr :=
   mkexpr (fun s => s x) (x :: nil) (var_expr_cond x).
 Coercion var_expr: V >-> expr.
 
+Proposition esub_cond (e: expr) (x: V) (e': expr) (s t : store):
+  eq_restr s t (remove Nat.eq_dec x (evar e) ++ evar e') ->
+  eval e (store_update s x (eval e' s)) =
+    eval e (store_update t x (eval e' t)).
+intro.
+assert (eval e' s = eval e' t).
+apply (econd e').
+intro; intro; apply H.
+apply in_or_app; right; assumption.
+rewrite <- H0.
+unfold store_update.
+apply (econd e).
+unfold eq_restr.
+intro; intro.
+destruct (Nat.eq_dec x x0).
+reflexivity.
+apply H; apply in_or_app; left.
+apply In_remove; assumption.
+Qed.
+Definition esub (e: expr) (x: V) (e': expr): expr :=
+  mkexpr (fun s => eval e (store_update s x (eval e' s)))
+    (remove Nat.eq_dec x (evar e) ++ evar e') (esub_cond e x e').
+
+Proposition esub_simpl (e: expr) (x: V) (e': expr):
+  ~In x (evar e) -> forall s, eval (esub e x e') s = eval e s.
+intros. simpl.
+apply econd. intro. intro.
+unfold store_update.
+destruct (Nat.eq_dec x x0).
+exfalso. apply H. rewrite e0. assumption.
+reflexivity.
+Qed.
+
 Proposition expr_eq (e1 e2: expr):
   (eval e1 = eval e2) -> (evar e1 = evar e2) -> e1 = e2.
 intros. destruct e1. destruct e2.
@@ -165,6 +207,7 @@ Qed.
 Definition const_guard (v: bool): guard :=
   mkguard (fun s => v) nil (const_guard_cond v).
 Coercion const_guard: bool >-> guard.
+
 Proposition equals_cond (e1 e2: expr) (s t : store):
   eq_restr s t (evar e1 ++ evar e2) ->
   (if Z.eq_dec (eval e1 s) (eval e2 s) then true else false) =
@@ -178,6 +221,29 @@ Qed.
 Definition equals (e1 e2: expr): guard :=
   mkguard (fun s => if Z.eq_dec (eval e1 s) (eval e2 s) then
     true else false) (evar e1 ++ evar e2) (equals_cond e1 e2).
+
+Proposition gsub_cond (g: guard) (x: V) (e: expr) (s t: store):
+  eq_restr s t (remove Nat.eq_dec x (gvar g) ++ evar e) ->
+  gval g (store_update s x (eval e s)) =
+  gval g (store_update t x (eval e t)).
+intro.
+assert (eval e s = eval e t).
+apply (econd e).
+intro; intro; apply H.
+apply in_or_app; right; assumption.
+rewrite <- H0.
+unfold store_update.
+apply (gcond g).
+unfold eq_restr.
+intro; intro.
+destruct (Nat.eq_dec x x0).
+reflexivity.
+apply H; apply in_or_app; left.
+apply In_remove; assumption.
+Qed.
+Definition gsub (g: guard) (x: V) (e: expr): guard :=
+  mkguard (fun s => gval g (store_update s x (eval e s)))
+    (remove Nat.eq_dec x (gvar g) ++ evar e) (gsub_cond g x e).
 
 Proposition guard_eq (g1 g2: guard):
   (gval g1 = gval g2) -> (gvar g1 = gvar g2) -> g1 = g2.
@@ -200,6 +266,7 @@ Inductive assert :=
 Coercion test: guard >-> assert.
 
 Definition lnot (p: assert): assert := (limp p false).
+Definition lequiv (p q: assert): assert := (land (limp p q) (limp q p)).
 Definition hasvaldash (e: expr): assert :=
   let y := fresh (evar e) in lexists y (hasval e y).
 Definition emp: assert := (lforall dummy (lnot (hasvaldash dummy))).
@@ -212,12 +279,87 @@ Definition hasval_alt (e e': expr): assert :=
 Definition hasvaldash_alt (e: expr): assert :=
   sand (pointstodash e) true.
 
+Fixpoint abound (p: assert): list V :=
+  match p with
+  | test g => nil
+  | hasval e e' => nil
+  | land p q => abound p ++ abound q
+  | lor p q => abound p ++ abound q
+  | limp p q => abound p ++ abound q
+  | lexists x p => x :: abound p
+  | lforall x p => x :: abound p
+  | sand p q => abound p ++ abound q
+  | simp p q => abound p ++ abound q
+  end.
+
+Fixpoint avar (p: assert): list V :=
+  match p with
+  | test g => gvar g
+  | hasval e e' => evar e ++ evar e'
+  | land p q => avar p ++ avar q
+  | lor p q => avar p ++ avar q
+  | limp p q => avar p ++ avar q
+  | lexists x p => remove Nat.eq_dec x (avar p)
+  | lforall x p => remove Nat.eq_dec x (avar p)
+  | sand p q => avar p ++ avar q
+  | simp p q => avar p ++ avar q
+  end.
+
+Definition aoccur (p: assert): list V := abound p ++ avar p.
+
+Definition Some_assert (p: assert): option assert := Some p.
+Coercion Some_assert: assert >-> option.
+
+Fixpoint asub (p: assert) (x: V) (e: expr): option assert :=
+  match p with
+  | test g => test (gsub g x e)
+  | hasval e1 e2 => hasval (esub e1 x e) (esub e2 x e)
+  | land p q => option_app (asub p x e) (fun ps =>
+      option_app (asub q x e) (fun qs => land ps qs))
+  | lor p q => option_app (asub p x e) (fun ps =>
+      option_app (asub q x e) (fun qs => lor ps qs))
+  | limp p q => option_app (asub p x e) (fun ps =>
+      option_app (asub q x e) (fun qs => limp ps qs))
+  | lexists y p => if Nat.eq_dec x y then lexists y p else
+      if in_dec Nat.eq_dec y (evar e) then None
+      else option_app (asub p x e) (fun ps => lexists y ps)
+  | lforall y p => if Nat.eq_dec x y then lforall y p else
+      if in_dec Nat.eq_dec y (evar e) then None
+      else option_app (asub p x e) (fun ps => lforall y ps)
+  | sand p q => option_app (asub p x e) (fun ps =>
+      option_app (asub q x e) (fun qs => sand ps qs))
+  | simp p q => option_app (asub p x e) (fun ps =>
+      option_app (asub q x e) (fun qs => simp ps qs))
+  end.
+
+Proposition asub_defined (p: assert) (x: V) (e: expr):
+  (forall x, In x (evar e) -> ~In x (abound p)) <-> exists q, asub p x e = Some q.
+induction p; simpl.
+- split; intros; auto.
+  exists (test (gsub g x e)); reflexivity.
+- split; intros; auto.
+  exists (hasval (esub e0 x e) (esub e1 x e)); reflexivity.
+- split; intros.
+  + apply In_app_split in H; destruct H.
+    apply IHp1 in H; destruct H.
+    apply IHp2 in H0; destruct H0.
+    exists (land x0 x1); rewrite H; rewrite H0; reflexivity.
+  + destruct H.
+    apply option_app_elim in H; destruct H; destruct H.
+    assert (exists q, asub p1 x e = Some q) by (exists x2; assumption).
+    apply option_app_elim in H1; destruct H1; destruct H1.
+    assert (exists q, asub p2 x e = Some q) by (exists x3; assumption).
+    apply not_In_split; split.
+    apply <- IHp1; assumption.
+    apply <- IHp2; assumption.
+Abort.
+
 Variant assignment :=
 | basic: V -> expr -> assignment
 | lookup: V -> expr -> assignment
 | mutation: V -> expr -> assignment
-| new: V -> expr -> assignment.
-(* TODO: dispose *)
+| new: V -> expr -> assignment
+| dispose: V -> assignment.
 
 Inductive program :=
 | assign: assignment -> program
@@ -243,6 +385,12 @@ Inductive bigstep: program -> heap * store -> option (heap * store) -> Prop :=
     ~(dom h n) ->
     bigstep (new x e) (h, s)
       (Some (heap_update h n (eval e s), store_update s x n))
+| step_dispose (x: V) (h: heap) (s: store):
+    dom h (s x) ->
+    bigstep (dispose x) (h, s) (Some (heap_clear h (s x), s))
+| step_dispose_fail (x: V) (h: heap) (s: store):
+    ~dom h (s x) ->
+    bigstep (dispose x) (h, s) None
 | step_comp (S1 S2: program) (h h' h'': heap) (s s' s'': store):
     bigstep S1 (h, s) (Some (h', s')) ->
     bigstep S2 (h', s') (Some (h'', s'')) ->
