src/Util.v
@@ -1,0 +1,88 @@
+(* Copyright 2022 Centrum Wiskunde & Informatica *)
+
+(* ON SEPERATION LOGIC *)
+(* Author: Hans-Dieter A. Hiep *)
+
+Require Export FunctionalExtensionality.
+Require Export PropExtensionality.
+Require Export Structures.Orders.
+Require Export List.
+Require Export Sorting.
+Require Export ZArith.
+
+Definition option_dec {T: Type} (o: option T): {exists x, o = Some x} + {o = None} :=
+  match o return ({exists x : T, o = Some x} + {o = None}) with
+  | Some t => left (ex_intro (fun x : T => Some t = Some x) t eq_refl)
+  | None => right eq_refl
+  end.
+
+Definition option_app {T1 T2: Type} (x: option T1) (f: T1 -> option T2): option T2 :=
+  match x with
+  | Some x => f x
+  | None => None
+  end.
+
+Proposition option_app_elim {T1 T2: Type} (x: option T1) (f: T1 -> option T2) (z: T2):
+  option_app x f = Some z -> exists y: T1, x = Some y /\ f y = Some z.
+intros. destruct x.
+simpl in H.
+exists t. split; auto.
+inversion H.
+Qed.
+
+Proposition In_remove (T: Type)
+    (eq_dec: forall (x y: T), {x = y} + {x <> y})
+    (x y: T) (xs: list T):
+  In x xs -> y <> x -> In x (remove eq_dec y xs).
+induction xs; intros; inversion H;
+simpl; destruct (eq_dec y a).
+exfalso. apply H0. rewrite <- H1. auto.
+rewrite H1. left. reflexivity.
+apply IHxs; assumption.
+right. apply IHxs; assumption.
+Qed.
+
+Proposition In_remove_elim (T: Type)
+    (eq_dec: forall (x y: T), {x = y} + {x <> y})
+    (x y: T) (xs: list T):
+  y <> x -> In x (remove eq_dec y xs) -> In x xs.
+induction xs; intros; simpl in H0.
+inversion H0.
+specialize (IHxs H).
+destruct (eq_dec y a).
+specialize (IHxs H0). right. assumption.
+inversion H0. rewrite H1. left. auto.
+specialize (IHxs H1). right. assumption.
+Qed.
+
+Proposition not_In_split (T: Type) (xs ys: list T) (x: T):
+  ~ In x (xs ++ ys) <-> ~ In x xs /\ ~ In x ys.
+split.
+intros; split; intro; apply H; apply in_or_app; auto.
+intros; destruct H; intro; apply in_app_or in H1; destruct H1; auto.
+Qed.
+
+Proposition In_app_split (T: Type) (xs ys zs: list T):
+  (forall x, In x xs -> ~ In x (ys ++ zs)) ->
+  (forall x, In x xs -> ~ In x ys) /\ (forall x, In x xs -> ~ In x zs).
+intros; split;
+intros; specialize H with x; apply H in H0;
+apply not_In_split in H0; destruct H0; auto.
+Qed.
+
+Proposition forall_iff_compat (T: Type) (P P': T -> Prop):
+  (forall x : T, P x <-> P' x) ->
+  (forall x : T, ~ P x) <-> (forall x : T, ~ P' x).
+intros; split; intro;
+intros; specialize H0 with x; intro;
+apply H0; apply H; assumption.
+Qed.
+
+Proposition forall2_iff_compat (T: Type) (P P': T -> T -> Prop):
+  (forall x y : T, P x y <-> P' x y) ->
+  (forall x y : T, ~ P x y) <-> (forall x y : T, ~ P' x y).
+intros; split; intro;
+intros; specialize H0 with x y; intro;
+apply H0; apply H; assumption.
+Qed.
+
